src/lowparse/pulse/LowParse.Pulse.VCList.fst
@@ -1,0 +1,199 @@
+module LowParse.Pulse.VCList
+include LowParse.Spec.VCList
+include LowParse.Pulse.Combinators
+open FStar.Tactics.V2
+open LowParse.Pulse.Util
+open Pulse.Lib.Stick
+open Pulse.Lib.Slice
+
+module SZ = FStar.SizeT
+module R = Pulse.Lib.Reference
+
+inline_for_extraction
+```pulse
+fn jump_nlist
+   (#t: Type0)
+   (#k: parser_kind)
+   (#p: parser k t)
+   (j: jumper p)
+   (n0: SZ.t)
+: jumper #(nlist (SZ.v n0) t) #(parse_nlist_kind (SZ.v n0) k) (tot_parse_nlist (SZ.v n0) p)
+=
+  (input: slice byte)
+  (offset0: SZ.t)
+  (#pm: perm)
+  (#v: Ghost.erased bytes)
+{
+  let mut pn = n0;
+  let mut poffset = offset0;
+  while (
+    let n = !pn;
+    (SZ.gt n 0sz)
+  ) invariant b . exists* n offset . (
+    pts_to input #pm v ** R.pts_to pn n ** R.pts_to poffset offset ** pure (
+    SZ.v offset <= Seq.length v /\ (
+    let pr0 = parse_consume (tot_parse_nlist (SZ.v n0) p) (Seq.slice v (SZ.v offset0) (Seq.length v)) in
+    let pr = parse_consume (tot_parse_nlist (SZ.v n) p) (Seq.slice v (SZ.v offset) (Seq.length v)) in
+    Some? pr0 /\ Some? pr /\
+    SZ.v offset0 + Some?.v pr0 == SZ.v offset + Some?.v pr /\
+    b == (SZ.v n > 0)
+  ))) {
+    let n = !pn;
+    let offset = !poffset;
+    tot_parse_nlist_eq (SZ.v n) p (Seq.slice v (SZ.v offset) (Seq.length v));
+    let offset' = j input offset;
+    pn := (SZ.sub n 1sz);
+    poffset := offset';
+  };
+  !poffset
+}
+```
+
+```pulse
+ghost
+fn nlist_cons_as_nondep_then
+  (#t: Type0)
+  (#k: parser_kind)
+  (#p: parser k t)
+  (s: serializer p { k.parser_kind_subkind == Some ParserStrong })
+  (n: pos)
+  (input: slice byte)
+  (#pm: perm)
+  (#v: nlist n t)
+requires
+  pts_to_serialized (tot_serialize_nlist n s) input #pm v
+ensures exists* v' .
+  pts_to_serialized (tot_serialize_nondep_then s (tot_serialize_nlist (n - 1) s)) input #pm v' **
+  (pts_to_serialized (tot_serialize_nondep_then s (tot_serialize_nlist (n - 1) s)) input #pm v' @==> pts_to_serialized (tot_serialize_nlist n s) input #pm v) **
+  pure (
+    v == (fst v' :: snd v')
+  )
+{
+  synth_inverse_1 t (n - 1);
+  synth_inverse_2 t (n - 1);
+  rewrite_with_stick
+    (pts_to_serialized (tot_serialize_nlist n s) input #pm v)
+    (pts_to_serialized (tot_serialize_synth _ (synth_nlist (n - 1)) (tot_serialize_nondep_then s (tot_serialize_nlist' (n - 1) s)) (synth_nlist_recip (n - 1)) ()) input #pm v);
+  pts_to_serialized_synth_l2r_stick
+    (tot_serialize_nondep_then s (tot_serialize_nlist' (n - 1) s))
+    (synth_nlist (n - 1))
+    (synth_nlist_recip (n - 1))
+    input;
+  stick_trans (pts_to_serialized (tot_serialize_nondep_then s (tot_serialize_nlist (n - 1) s)) input #pm _) _ _
+}
+```
+
+inline_for_extraction
+```pulse
+fn nlist_hd
+  (#t: Type0)
+  (#k: parser_kind)
+  (#p: parser k t)
+  (s: serializer p { k.parser_kind_subkind == Some ParserStrong })
+  (j: jumper p)
+  (n: pos)
+  (input: slice byte)
+  (#pm: perm)
+  (#v: Ghost.erased (nlist n t))
+requires
+  pts_to_serialized (tot_serialize_nlist n s) input #pm v
+returns input' : slice byte
+ensures exists* v' .
+  pts_to_serialized s input' #pm v' **
+  (pts_to_serialized s input' #pm v' @==> pts_to_serialized (tot_serialize_nlist n s) input #pm v) **
+  pure (
+    Cons? v /\
+    v' == List.Tot.hd v
+  )
+{
+  nlist_cons_as_nondep_then s n input;
+  let res = nondep_then_fst s j (tot_serialize_nlist (n - 1) s) input;
+  stick_trans (pts_to_serialized s res #pm _) _ _;
+  res
+}
+```
+
+inline_for_extraction
+```pulse
+fn nlist_tl
+  (#t: Type0)
+  (#k: parser_kind)
+  (#p: parser k t)
+  (s: serializer p { k.parser_kind_subkind == Some ParserStrong })
+  (j: jumper p)
+  (n: pos)
+  (input: slice byte)
+  (#pm: perm)
+  (#v: Ghost.erased (nlist n t))
+requires
+  pts_to_serialized (tot_serialize_nlist n s) input #pm v
+returns input' : slice byte
+ensures exists* v' .
+  pts_to_serialized (tot_serialize_nlist (n - 1) s) input' #pm v' **
+  (pts_to_serialized (tot_serialize_nlist (n - 1) s) input' #pm v' @==> pts_to_serialized (tot_serialize_nlist n s) input #pm v) **
+  pure (
+    Cons? v /\
+    v' == List.Tot.tl v
+  )
+{
+  nlist_cons_as_nondep_then s n input;
+  let res = nondep_then_snd s j (tot_serialize_nlist (n - 1) s) input;
+  stick_trans (pts_to_serialized (tot_serialize_nlist (n - 1) s) res #pm _) _ _;
+  res
+}
+```
+
+inline_for_extraction
+```pulse
+fn nlist_nth
+   (#t: Type0)
+   (#k: parser_kind)
+   (#p: parser k t)
+   (s: serializer p { k.parser_kind_subkind == Some ParserStrong })
+   (j: jumper p)
+   (n0: SZ.t)
+  (input: slice byte)
+  (#pm: perm)
+  (#v0: Ghost.erased (nlist (SZ.v n0) t))
+  (i0: SZ.t { SZ.v i0 < SZ.v n0 })
+requires
+  pts_to_serialized (tot_serialize_nlist (SZ.v n0) s) input #pm v0
+returns input' : slice byte
+ensures exists* v .
+  pts_to_serialized s input' #pm v **
+  (pts_to_serialized s input' #pm v @==> pts_to_serialized (tot_serialize_nlist (SZ.v n0) s) input #pm v0) **
+  pure (v == List.Tot.index v0 (SZ.v i0))
+{
+  stick_id (pts_to_serialized (tot_serialize_nlist (SZ.v n0) s) input #pm v0);
+  let mut pi = 0sz;
+  let mut pres = input;
+  while (
+    let i = !pi;
+    (SZ.lt i i0)
+  ) invariant b . exists* i res (n: nat) (v: nlist n t) . (
+    R.pts_to pi i ** R.pts_to pres res **
+    pts_to_serialized (tot_serialize_nlist n s) res #pm v **
+    (pts_to_serialized (tot_serialize_nlist n s) res #pm v @==> pts_to_serialized (tot_serialize_nlist (SZ.v n0) s) input #pm v0) **
+    pure (
+      SZ.v i <= SZ.v i0 /\
+      (b == (SZ.v i < SZ.v i0)) /\
+      n == SZ.v n0 - SZ.v i /\
+      List.Tot.index v0 (SZ.v i0) == List.Tot.index v (SZ.v i0 - SZ.v i)
+  )) {
+    let res = !pres;
+    let i = !pi;
+    let res2 = nlist_tl s j (SZ.v n0 - SZ.v i) res;
+    pi := (SZ.add i 1sz);
+    pres := res2;
+    stick_trans
+      (pts_to_serialized (tot_serialize_nlist (SZ.v n0 - SZ.v i - 1) s) res2 #pm _)
+      _
+      _
+  };
+  let res = !pres;
+  let res2 = nlist_hd s j (SZ.v n0 - SZ.v i0) res;
+  stick_trans
+    (pts_to_serialized s res2 #pm _) _ _;
+  res2
+}
+```
